# 5.  Predicate Logic
_21/10/22_
*Lecture conducted by a tutor*

Prove propositions using tactics
- assume & applying for \to, ¬
- constructor & cases for ^
- left/right & cases for v
- constructor for true
- cases for false
Intuitonistic logic: prove theorems by combining...
Classical logic: use magic (em & raa)

## Types

`#check ℕ` - `\bn`, natural numbers 0,1,2,....
`#check bool` - tt,ff
`#check list ℕ`


Types are like sets
Types have terms (*elements*)
```lean
#check 3
#check tt
#check [3,4,5]
```

## Predicates and Relations

### Predicates (*properties of elements*)
Prime : ℕ → Prop
Prime 3 : -- Prop, Prime 4: Prop
isZero : ℕ → Prop

```lean
def isZero : ℕ → Prop | 0 := true | _ := false
#check isZero
#check isZero 0
#check isZero 4
#check isZero 3
```

### Relations (*Predicates with several inputs*)
le : ℕ → (ℕ → Prop)
le 2 3 means 2 is less or equal to 3

```lean
#check 2 ≤ 3
#check 5 ≤ 3
```

A relation for every type: equality
```lean
#check 3 = 3
#check 3 = 4
```

`namespace social` - Non-mathematical example: type of social media access
`constant Account : Type` - Predicate: is this account a bot?
`constant isBot : Account → Prop` - Relation: the 'follows' relation follows acc1 acc2 means that acc1 follows acc2

```lean
constant follows : Account → Account → Prop
constant account1 : Account
constant account2 : Account
#check account1 = account2
```
## Quantifiers

∀ : universal quantifier (`\forall`)
`#check ∀ x : Account , isBot x`

∃ : existential quanitifier (`\exists`)
`#check ∃ x : Account, isBot x`

Can use quantifiers in definition

```lean
def haveCommonFollower (acc1 acc2 : Account) : Prop
  := ∃ acc3 : Account, follows acc3 acc1 ∧ follows acc3 acc2
#check haveCommonFollower

def fakeFollowing (acc : Account) : Prop
  := ∀ acc' : Account, follows acc' acc → isBot acc'
#check fakeFollowing

end social
```


∀ x : A, (∃ x : A ..x..) .. x ..
scope, shadowing

```lean
variables A B C : Type
variables P Q R : Prop
variables PP QQ : A → Prop

example : (∀ x : A, PP x) → (∀ y : A, PP y → QQ y) → (∀ z : A, QQ z) :=

begin
  assume h g z,
  apply g,
  apply h,
end


example : (∃ x : A, PP x) → (∀ y : A, PP y → QQ y) → (∃ z : A, QQ z) :=
begin
  assume h g,
  cases h with z pz,
  existsi z,
  apply g,
  exact pz,
end
```

## Example Proofs
```lean
example : (∀ x : A, PP x ∧ QQ x) ↔ (∀ x : A, PP x) ∧ (∀ x : A, QQ x) :=
begin
  constructor,
  assume h,
  constructor,
  assume x,
  have f : PP x ∧ QQ x,
  apply h,
  cases f with px qx,
  exact px,
  assume x,
  have f: PP x ∧ QQ x,
  apply h,
  cases f with px qx,
  exact qx,
  assume h x,
  cases h with Px Qx,
  constructor,
  apply Px,
  apply Qx,
end
```