# 5. Applicative Functors
_20/02/23_

## Generalising fmap

```haskell
fmap0 :: a -> f a 
fmap1 :: (a -> b) -> f a -> f b
fmap2 :: (a -> b -> c) -> f a -> f b -> f c
fmap3 :: (a -> b -> c -> d) -> f a -> f b -> f c -> f d
```


```haskell
pure :: a-> f a -- Turn a value into a data strucutre. 
((*)) :: f (a -> b) -> f a -> f b --() is a prefix operator. Need to give brackets when defining it as a type. Generalised form of function applicaiton

pure g (*) x (*) y (*) z -- applicative style

(*) -- does it to the left

fmap0 :: a -> f a
fmap0 = pure 

fmap1 :: (a -> b) -> f a -> f b
fmap1 g x = pure g (*) x

fmap2 :: (a -> b -> c) -> f a -> f b -> f c
fmap2 g x y = (pure g (*) x ) (*) y
```

## Applicative Functors
```haskell
class Functor f => Applicative f where
	pure :: a -> f a
	((*)) :: f(a->b) -> f a -> f b
```

### Example: Maybe

```haskell
instance Applicative Maybe where
	-- pure :: a -> Maybe a
	pure x = Just x
	-- ((*)) :: maybe (a->b) -> Maybe a -> Maybe b
	Nothing (*) mx = Nothing
	(Just g) (*) mx = fmap g mx
```

### Example: Lists

```haskell
instance Applicative [] where
	-- pure :: a -> [a]
	pure x = [x]
	-- ((*)) :: [a->b] -> [a] -> [b]
	gs (*) xs = [g x | g <- gs, x <- xs] 
```
